add bilSimps
also selftest that test whether it loads and Holmakefile added.

The bilSimps just collects the most basic rewrites, which I believe are
save and often useful.

bilSimps.sig
@@ -1,0 +1,13 @@
+signature bilSimps =
+sig
+   include Abbrev
+
+   (* Rewrite rules for all the types defined as part of the bil formalisation. *)
+   val bil_TYPES_ss : simpLib.ssfrag;
+
+   (* Simple rewrites *)
+   val bil_SIMPLE_REWRS_ss : simpLib.ssfrag
+
+   (* All bil stuff *)
+   val bil_ss : simpLib.ssfrag
+end
