bilSimps.sml
@@ -1,0 +1,204 @@
+structure bilSimps :> bilSimps =
+struct
+
+open HolKernel boolLib liteLib simpLib Parse bossLib;
+open bilTheory;
+open bil_auxiliaryTheory bil_immTheory bil_valuesTheory;
+open bil_imm_expTheory bil_mem_expTheory bil_envTheory;
+open bil_expTheory bil_programTheory bil_typingTheory;
+
+val bil_list_of_types = [
+   mk_thy_type {Tyop="bil_imm_t",            Thy="bil_imm", Args=[]},
+   mk_thy_type {Tyop="bil_immtype_t",        Thy="bil_imm", Args=[]},
+
+   mk_thy_type {Tyop="bil_unary_exp_t",      Thy="bil_imm_exp", Args=[]},
+   mk_thy_type {Tyop="bil_bin_exp_t",        Thy="bil_imm_exp", Args=[]},
+   mk_thy_type {Tyop="bil_bin_pred_t",       Thy="bil_imm_exp", Args=[]},
+   mk_thy_type {Tyop="bil_cast_t",           Thy="bil_imm_exp", Args=[]},
+
+   mk_thy_type {Tyop="bil_endian_t",         Thy="bil_mem_exp", Args=[]},
+
+   mk_thy_type {Tyop="bil_val_t",            Thy="bil_values", Args=[]},
+   mk_thy_type {Tyop="bil_type_t",           Thy="bil_values", Args=[]},
+
+   mk_thy_type {Tyop="bil_var_t",            Thy="bil_env", Args=[]},
+   mk_thy_type {Tyop="bil_var_environment_t",Thy="bil_env", Args=[]},
+   mk_thy_type {Tyop="bil_env_cond_t",       Thy="bil_env", Args=[]},
+
+   mk_thy_type {Tyop="bil_label_t",          Thy="bil_program", Args=[]},
+   mk_thy_type {Tyop="bil_stmt_t",           Thy="bil_program", Args=[]},
+   mk_thy_type {Tyop="bil_block_t",          Thy="bil_program", Args=[]},
+   mk_thy_type {Tyop="bil_program_t",        Thy="bil_program", Args=[]},
+   mk_thy_type {Tyop="bil_programcounter_t", Thy="bil_program", Args=[]},
+   mk_thy_type {Tyop="bil_termcode_t",       Thy="bil_program", Args=[]},
+   mk_thy_type {Tyop="bil_state_t",          Thy="bil_program", Args=[]}
+];
+
+
+
+val bil_TYPES_ss = rewrites (flatten (map type_rws bil_list_of_types))
+
+val bil_SIMPLE_REWRS_imm = rewrites [
+  type_of_bil_imm_def,
+  type_of_n2bs,
+  type_of_n2b_fixed,
+  type_of_w2bs,
+  type_of_bool2b,
+  type_of_v2bs,
+  w2bs_REWRS,
+  v2bs_REWRS,
+  b2v_def,
+  v2n_b2v,
+
+  n2bs_b2n,
+  b2n_def,
+  n2bs_def,
+  b2w_REWRS,
+  w2bs_REWRS,
+  w2bs_b2w,
+  v2n_w2v,
+  bool2b_inv,
+  wordsTheory.n2w_w2n,
+
+  size_of_bil_immtype_INJ,
+  size_of_bil_immtype_NEQ_0,
+  is_valid_bil_immtype_size_IMP,
+  bil_immtype_of_num_inv 
+];
+
+
+val bil_SIMPLE_REWRS_env = rewrites [
+  bil_var_name_def,
+  bil_var_type_def,
+  is_env_regular_def,
+  is_valid_env_empty,
+  bil_env_write_Irregular,
+  bil_env_write_Irregular_WrongVal
+]
+
+
+
+
+val bil_SIMPLE_REWRS_imm_exp = rewrites [
+  bil_unary_exp_GET_OPER_def,
+  bil_bin_exp_GET_OPER_def,
+  bil_bin_pred_GET_OPER_def,
+  bil_gencast_def,
+  bil_unary_exp_REWRS,
+  bil_bin_exp_REWRS,
+
+  type_of_bil_unary_exp,
+  type_of_bil_unary_exps,
+  bil_unary_exps_REWRS,
+  type_of_bil_bin_exp,
+  type_of_bil_bin_exps,
+  bil_bin_exps_REWRS,
+  bil_bin_pred_REWRS,
+  bil_bin_preds_REWRS,
+
+  bil_cast_REWRS,
+  bil_lcast_def,
+  bil_hcast_REWRS,
+  bil_scast_REWRS,
+
+  type_of_bil_gencast,
+  bil_gencast_ID,
+  bil_casts_ID,
+  bil_casts_Bit1,
+  type_of_bil_casts
+];
+
+
+val bil_SIMPLE_REWRS_mem_exp = rewrites [
+  bil_number_of_mem_splits_REWRS,
+  bil_number_of_mem_splits_NEQ_SOME0,
+  bil_number_of_mem_splits_ID,
+  bil_number_of_mem_splits_EQ_SOME1,
+
+  type_of_bil_mem_concat,
+  type_of_bil_load_from_mem,
+  bil_load_from_mem_NONE_REWRS,
+  bil_load_from_mem_EQ_NONE_IMP,
+
+  bil_load_from_mem_used_addrs_REWRS,
+  bil_load_from_mem_used_addrs_FINITE,
+  bil_load_from_mem_used_addrs_EMPTY,
+
+  bil_store_in_mem_NONE_REWRS,
+  bil_store_in_mem_EQ_NONE_IMP,
+  bil_store_in_mem_used_addrs_REWRS,
+  bil_store_in_mem_used_addrs_FINITE,
+  bil_store_in_mem_used_addrs_EMPTY
+];
+  
+
+
+val bil_SIMPLE_REWRS_mem_exp = rewrites [
+  bil_number_of_mem_splits_REWRS,
+  bil_number_of_mem_splits_NEQ_SOME0,
+  bil_number_of_mem_splits_ID,
+  bil_number_of_mem_splits_EQ_SOME1,
+
+  type_of_bil_mem_concat,
+  type_of_bil_load_from_mem,
+  bil_load_from_mem_NONE_REWRS,
+  bil_load_from_mem_EQ_NONE_IMP,
+
+  bil_load_from_mem_used_addrs_REWRS,
+  bil_load_from_mem_used_addrs_FINITE,
+  bil_load_from_mem_used_addrs_EMPTY,
+
+  bil_store_in_mem_NONE_REWRS,
+  bil_store_in_mem_EQ_NONE_IMP,
+  bil_store_in_mem_used_addrs_REWRS,
+  bil_store_in_mem_used_addrs_FINITE,
+  bil_store_in_mem_used_addrs_EMPTY
+];
+  
+
+val bil_SIMPLE_REWRS_values = rewrites [
+  bil_val_checker_REWRS,
+  type_of_bil_val_def,
+  bil_type_checker_REWRS,
+  bil_type_is_BoolType_IMPL
+];
+
+val bil_SIMPLE_REWRS_exp = rewrites [
+  bil_eval_exp_def,
+  bil_eval_cast_REWRS,
+  bil_eval_unary_exp_REWRS,
+  bil_eval_bin_exp_REWRS,
+  bil_eval_bin_pred_REWRS,
+  bil_eval_ifthenelse_REWRS,
+  bil_eval_ifthenelse_REWRS_Unknown,
+  bil_eval_load_Unknown_REWRS,
+  bil_eval_store_Unknown_REWRS
+];
+
+val bil_SIMPLE_REWRS_program = rewrites [
+  bil_stmt_to_string_def,
+  r2s_REWRS,
+  bil_state_is_terminated_IMP,
+  bil_declare_initial_value_def
+];
+
+val bil_SIMPLE_REWRS_typing = rewrites [
+  type_of_bil_exp_EQ_SOME_REWRS,
+  type_of_bil_exp_EQ_NONE_REWRS
+];
+
+val bil_SIMPLE_REWRS_ss = simpLib.merge_ss [
+  bil_TYPES_ss,
+  bil_SIMPLE_REWRS_imm,
+  bil_SIMPLE_REWRS_values,
+  bil_SIMPLE_REWRS_env,
+  bil_SIMPLE_REWRS_imm_exp,
+  bil_SIMPLE_REWRS_mem_exp,
+  bil_SIMPLE_REWRS_exp,
+  bil_SIMPLE_REWRS_program,
+  bil_SIMPLE_REWRS_typing
+];
+
+val bil_ss = bil_SIMPLE_REWRS_ss;
+
+end
