selftest.sml
@@ -1,0 +1,11 @@
+open HolKernel Parse boolTheory boolLib pairTheory
+
+open bilSimps bilTheory;
+open bil_auxiliaryTheory bil_immTheory bil_valuesTheory;
+open bil_imm_expTheory bil_mem_expTheory bil_envTheory;
+open bil_expTheory bil_programTheory bil_typingTheory;
+
+
+
+
+val _ = Process.exit Process.success;
